thy/OpenFlow/OpenFlowDoc.thy
@@ -392,7 +392,7 @@ text\<open>Thus, @{const generalized_fw_join} has a number of applications.
 For example, it could be used to compute a firewall ruleset that represents two firewalls that are executed in sequence.
 \<close>
 definition "simple_action_conj a b \<equiv> (if a = simple_action.Accept \<and> b = simple_action.Accept then simple_action.Accept else simple_action.Drop)"
-definition "simple_rule_conj \<equiv> (split SimpleRule \<circ> apsnd (split simple_action_conj))"
+definition "simple_rule_conj \<equiv> (uncurry SimpleRule \<circ> apsnd (uncurry simple_action_conj))"
 theorem "simple_fw rs\<^sub>1 p = Decision FinalAllow \<and> simple_fw rs\<^sub>2 p = Decision FinalAllow \<longleftrightarrow>
 simple_fw (map simple_rule_conj (generalized_fw_join (map simple_rule_dtor rs\<^sub>1) (map simple_rule_dtor rs\<^sub>2))) p = Decision FinalAllow"
 unfolding simple_rule_conj_def simple_action_conj_def[abs_def] using simple_fw_join by(force simp add: comp_def apsnd_def map_prod_def case_prod_unfold)
